Foundation/Modal/ZeroSubstitution.lean
@@ -2,15 +2,15 @@ import Foundation.Modal.Letterless
 
 namespace LO.Modal
 
-def ZeroSubstitution (α) := {s : Substitution α // ∀ {a : α}, ((.atom a)⟦s⟧).letterless }
+def ZeroSubstitution (α) := {s : Substitution α // ∀ {a : α}, ((.atom a)⟦s⟧).Letterless }
 
-lemma Formula.letterless_zeroSubst {φ : Formula α} {s : ZeroSubstitution α} : (φ⟦s.1⟧).letterless := by
-  induction φ <;> simp [Formula.letterless, *];
+lemma Formula.Letterless_zeroSubst {φ : Formula α} {s : ZeroSubstitution α} : (φ⟦s.1⟧).Letterless := by
+  induction φ <;> simp [Formula.Letterless, *];
   case hatom => exact s.2;
 
-lemma Formula.toModalFormula.letterless {φ : Propositional.Formula α} (h : φ.letterless) : φ.toModalFormula.letterless := by
-  induction φ using Propositional.Formula.rec' <;> simp_all [Propositional.Formula.letterless, Formula.letterless];
+lemma Formula.toModalFormula.Letterless {φ : Propositional.Formula α} (h : φ.Letterless) : φ.toModalFormula.Letterless := by
+  induction φ using Propositional.Formula.rec' <;> simp_all [Propositional.Formula.Letterless, Formula.Letterless];
 
-instance : Coe (Propositional.ZeroSubstitution α) (Modal.ZeroSubstitution α) := ⟨λ ⟨s, p⟩ => ⟨λ φ => s φ, λ {_} => Formula.toModalFormula.letterless p⟩⟩
+instance : Coe (Propositional.ZeroSubstitution α) (Modal.ZeroSubstitution α) := ⟨λ ⟨s, p⟩ => ⟨λ φ => s φ, λ {_} => Formula.toModalFormula.Letterless p⟩⟩
 
 end LO.Modal
